src/Examples/ABC/VProgram/SynthesizedPortion.cs
@@ -3,7 +3,6 @@ public class SynthesizedPortion
     public static void SynthesizedSequence()
     {
           CST.Message C1 = PoirotMain.Nondet.Message();
-          CST.Message C2 = ((ABC.B)GlobalObjectsForCST.B).invoke(C1);
-          CST.Message C3 = ((ABC.C)GlobalObjectsForCST.C).invoke(C2);
+          CST.Message C2 = ((ABC.C)GlobalObjectsForCST.C).invoke(C1);
     }
 }
